lakefile.lean
@@ -4,5 +4,8 @@ open Lake DSL
 
 package maze
 
+require aesop from git "https://github.com/leanprover-community/aesop" @ "v4.4.0"
+
+
 @[default_target]
 lean_lib Maze
